$$
mv_0=m(v_1+v_2)
$$

$$
F-\frac{B^2L^2(v_1-v_2)}{R}=ma_1\\
\frac{B^2L^2(v_1-v_2)}{R}=ma_2
$$

$$
E=\frac{\triangle \varphi }{\triangle t}=\frac{\triangle B }{\triangle t}S+B'lv
$$

$$
有外力电容
\\\left \{ \begin{array}{l}I=\frac{\triangle q}{\triangle t}\\ \triangle q=C\triangle U\\\triangle U=Bl\triangle v\\ a=\frac{\triangle v}{\triangle t} \end{array}\right.\Rightarrow I=BlCa\\
ma=F-BIl=F-B^2L^2Ca\Rightarrow a=\frac{F}{m-B^2L^2C}\triangle
$$

$$
无外力电容\\E=\frac QC=BLv\Rightarrow v=\frac{Q}{BLC}
\\BIL\triangle t=mv-mv_0=BLQ
$$

